oqergnwrjgn

.lake/build/ir/Games/gameLib_fixfix/Pairing.c
@@ -13,6 +13,51 @@
 #ifdef __cplusplus
 extern "C" {
 #endif
+LEAN_EXPORT lean_object* l___private_Games_gameLib__fixfix_Pairing_0__History__on__turn_match__1_splitter___rarg___boxed(lean_object*, lean_object*, lean_object*);
+LEAN_EXPORT lean_object* l___private_Games_gameLib__fixfix_Pairing_0__History__on__turn_match__1_splitter(lean_object*);
+LEAN_EXPORT lean_object* l___private_Games_gameLib__fixfix_Pairing_0__History__on__turn_match__1_splitter___rarg(lean_object*, lean_object*, lean_object*);
+uint8_t lean_nat_dec_eq(lean_object*, lean_object*);
+lean_object* lean_nat_sub(lean_object*, lean_object*);
+LEAN_EXPORT lean_object* l___private_Games_gameLib__fixfix_Pairing_0__History__on__turn_match__1_splitter___rarg(lean_object* x_1, lean_object* x_2, lean_object* x_3) {
+_start:
+{
+lean_object* x_4; uint8_t x_5; 
+x_4 = lean_unsigned_to_nat(0u);
+x_5 = lean_nat_dec_eq(x_1, x_4);
+if (x_5 == 0)
+{
+lean_object* x_6; lean_object* x_7; lean_object* x_8; 
+x_6 = lean_unsigned_to_nat(1u);
+x_7 = lean_nat_sub(x_1, x_6);
+x_8 = lean_apply_1(x_3, x_7);
+return x_8;
+}
+else
+{
+lean_dec(x_3);
+lean_inc(x_2);
+return x_2;
+}
+}
+}
+LEAN_EXPORT lean_object* l___private_Games_gameLib__fixfix_Pairing_0__History__on__turn_match__1_splitter(lean_object* x_1) {
+_start:
+{
+lean_object* x_2; 
+x_2 = lean_alloc_closure((void*)(l___private_Games_gameLib__fixfix_Pairing_0__History__on__turn_match__1_splitter___rarg___boxed), 3, 0);
+return x_2;
+}
+}
+LEAN_EXPORT lean_object* l___private_Games_gameLib__fixfix_Pairing_0__History__on__turn_match__1_splitter___rarg___boxed(lean_object* x_1, lean_object* x_2, lean_object* x_3) {
+_start:
+{
+lean_object* x_4; 
+x_4 = l___private_Games_gameLib__fixfix_Pairing_0__History__on__turn_match__1_splitter___rarg(x_1, x_2, x_3);
+lean_dec(x_2);
+lean_dec(x_1);
+return x_4;
+}
+}
 lean_object* initialize_Init(uint8_t builtin, lean_object*);
 lean_object* initialize_Games_gameLib__fixfix_Positional(uint8_t builtin, lean_object*);
 static bool _G_initialized = false;
